IrisCore/Own.thy
@@ -1,0 +1,67 @@
+theory Own
+imports ProofRules
+begin
+
+context inG begin
+definition own :: "gname \<Rightarrow> 'b \<Rightarrow> 'a upred_f" where
+  "own \<gamma> x = upred_own (put_cmra \<gamma> x)"
+
+lemma own_ne [upred_ne_rule]: "n_equiv n x y \<Longrightarrow> n_equiv n (own \<gamma> x) (own \<gamma> y)" 
+  unfolding own_def
+  apply (rule upred_own_ne)
+  using non_expansiveE[OF put_ne] by simp
+
+lemma own_valid: "own \<gamma> a \<turnstile> \<V>(a)"
+  unfolding own_def
+  apply (rule upred_entails_trans[OF upred_own_valid])
+  by (auto simp: upred_entails.rep_eq upred_valid.rep_eq put_n_valid)
+
+lemma own_op: "own \<gamma> (a\<cdot>b) \<stileturn>\<turnstile> own \<gamma> a \<^emph> own \<gamma> b"
+  unfolding own_def put_op
+  by (rule upred_own_op)
+
+lemma own_valid2: "own \<gamma> a1 -\<^emph> own \<gamma> a2 -\<^emph> \<V>(a1\<cdot>a2)"
+  unfolding own_def
+  apply (rule upred_wand_holds2I)
+  apply (rule upred_entails_trans[OF upred_wand_holds2E[OF upred_own_valid2]])
+  by (auto simp: upred_entails.rep_eq upred_valid.rep_eq put_n_valid put_op[symmetric])
+
+lemma own_alloc: "valid a \<Longrightarrow> \<Rrightarrow>\<^sub>b (own \<gamma> a)"
+  sorry (* Axiomatized as proof in Coq is not easily reproducible. *)
+  
+lemma own_update: "put_cmra \<gamma> a\<leadsto>{put_cmra \<gamma> b} \<Longrightarrow> own \<gamma> a ==\<^emph> own \<gamma> b"
+  unfolding camera_upd_def own_def
+  apply (rule upred_wand_holdsI)
+  apply transfer'
+  apply auto
+  by (metis n_incl_refl n_valid_incl_subst)
+
+lemma add_own: "\<lbrakk>valid a; Q\<^emph>(own \<gamma> a)\<turnstile>\<Rrightarrow>\<^sub>bR\<rbrakk> \<Longrightarrow> Q\<turnstile>\<Rrightarrow>\<^sub>bR"
+proof -
+  assume assms: "valid a" "Q\<^emph>(own \<gamma> a)\<turnstile>\<Rrightarrow>\<^sub>bR"
+  from own_alloc[OF this(1)] have "\<Rrightarrow>\<^sub>b own \<gamma> a" .
+  from assms(2) have "Q\<^emph>\<Rrightarrow>\<^sub>b own \<gamma> a\<turnstile>\<Rrightarrow>\<^sub>b R"
+    by (meson upd_frameR upd_mono upd_idem upred_entails_trans)
+  from add_holds[OF \<open>\<Rrightarrow>\<^sub>b own \<gamma> a\<close> this] show ?thesis .
+qed  
+end
+
+notation inG.own ("own _ _ _")
+
+context fixes get_cmra :: "gname \<Rightarrow> 'a::ucamera \<Rightarrow> 'b::total_camera option"
+  and put_cmra :: "gname \<Rightarrow> 'b \<Rightarrow> 'a"
+  assumes inG: "inG get_cmra put_cmra"
+begin
+lemma own_core_persis: "own put_cmra \<gamma> a \<turnstile> \<box>(own put_cmra \<gamma> (core a))"
+  unfolding inG.own_def[OF inG]
+  apply (rule upred_entails_trans[OF upred_own_core_persis])
+  unfolding core_def
+  apply (auto simp: comp_def inG.put_pcore[OF inG])
+  using total_pcore
+  by (metis option.case_eq_if option.distinct(1) upred_entails_refl)
+
+lemma pcore_id_put: "pcore_id_pred x \<Longrightarrow> pcore_id_pred (put_cmra \<gamma> x)"
+  unfolding pcore_id_pred_def inG.put_pcore[OF inG]
+  by auto
+end
+end
